code/experimental/rsa/Hacl.Impl.Shift.fst
@@ -18,18 +18,19 @@ let bn_tbit = u64 0x8000000000000000
 
 val bn_lshift1_:
   aLen:size_t ->
-  a:lbignum aLen -> carry:uint64 -> i:size_t{v i <= v aLen} ->
+  a:lbignum aLen -> carry:lbignum (size 1) ->
   res:lbignum aLen -> Stack unit
-  (requires (fun h -> live h a /\ live h res))
-  (ensures (fun h0 _ h1 -> preserves_live h0 h1 /\ modifies1 res h0 h1))
-  [@"c_inline"]
-let rec bn_lshift1_ aLen a carry i res =
-  if (i <. aLen) then begin
+  (requires (fun h -> live h a /\ live h res /\ live h carry))
+  (ensures (fun h0 _ h1 -> preserves_live h0 h1 /\ modifies2 carry res h0 h1))
+  [@ "substitute"]
+let bn_lshift1_ aLen a carry res =
+  let h0 = FStar.HyperStack.ST.get() in
+  loop2_simple #h0 aLen carry res
+  (fun i ->
     let tmp = a.(i) in
-    res.(i) <- (shift_left #U64 tmp (u32 1)) |. carry;
-    let carry = if (eq_u64 (logand #U64 tmp bn_tbit) bn_tbit) then u64 1 else u64 0 in
-    bn_lshift1_ aLen a carry (add #SIZE i (size 1)) res
-  end
+    res.(i) <- (shift_left #U64 tmp (u32 1)) |. carry.(size 0);
+    carry.(size 0) <- if (eq_u64 (logand #U64 tmp bn_tbit) bn_tbit) then u64 1 else u64 0
+  )
 
 // res = a << 1
 val bn_lshift1:
@@ -38,23 +39,31 @@ val bn_lshift1:
   (requires (fun h -> live h a /\ live h res))
   (ensures (fun h0 _ h1 -> preserves_live h0 h1 /\ modifies1 res h0 h1))
   [@"c_inline"]
-let bn_lshift1 aLen a res = bn_lshift1_ aLen a (u64 0) (size 0) res
+let bn_lshift1 aLen a res =
+  let h0 = FStar.HyperStack.ST.get () in
+  alloc1 #h0 (size 1) (u64 0) res
+  (fun h -> (fun _ r -> True))
+  (fun carry ->
+    bn_lshift1_ aLen a carry res
+  )
 
 val bn_pow2_mod_n_:
   aLen:size_t -> a:lbignum aLen ->
-  i:size_t -> p:size_t ->
+  p:size_t ->
   rLen:size_t{v aLen < v rLen} -> res:lbignum rLen ->
   Stack unit
     (requires (fun h -> live h a /\ live h res /\ disjoint res a))
     (ensures (fun h0 _ h1 -> preserves_live h0 h1 /\ modifies1 res h0 h1))
-  [@"c_inline"]
-let rec bn_pow2_mod_n_ aLen a i p rLen res =
-  if (i <. p) then begin
+  [@ "substitute"]
+let bn_pow2_mod_n_ aLen a p rLen res =
+  iteri_simple #uint64 #(v rLen) p
+  (fun i res ->
+    let h = FStar.HyperStack.ST.get() in
+    assume (live h res /\ live h a);
     bn_lshift1 rLen res res;
     (if not (bn_is_less rLen res aLen a) then
-      let _ = bn_sub rLen res aLen a res in ());
-    bn_pow2_mod_n_ aLen a (add #SIZE i (size 1)) p rLen res
-  end
+      let _ = bn_sub rLen res aLen a res in ())
+  ) res
 
 // res = 2 ^^ p % a
 val bn_pow2_mod_n:
@@ -75,7 +84,7 @@ let bn_pow2_mod_n aLen aBits a p res =
     assume (v aBits / 64 < v rLen);
     bn_set_bit rLen tmp aBits;
     let _ = bn_sub rLen tmp aLen a tmp in // tmp = tmp - a
-    bn_pow2_mod_n_ aLen a aBits p rLen tmp;
+    bn_pow2_mod_n_ aLen a (sub #SIZE p aBits) rLen tmp;
     let tmp' = Buffer.sub tmp (size 0) aLen in
     copy res aLen tmp'
   )
